fixes

proof/memory_map.bpl
@@ -1,70 +1,49 @@
-var mem: mem_t;
+const NULL: uint8_ptr_t;              axiom NULL == 0bv64;
 
-const NULL: uint8_ptr_t;
-axiom NULL == 0bv64;
+var send_buf: mem_t; //from 417792bv64 to 421888bv64
+const send_buf_size: uint64_t;        axiom send_buf_size == 4096bv64;
+const send_buf_ptr_low: uint8_ptr_t;  axiom send_buf_ptr_low == 417792bv64;
+const send_buf_ptr_high: uint8_ptr_t; axiom send_buf_ptr_high == 421888bv64;
+function {:inline} AddrInSendBuf(ptr: bv64): bool { GE_64(ptr, send_buf_ptr_low) && LT_64(ptr, send_buf_ptr_high) }
 
-/*
-static sir_channel_context_t sir_channel_context;
-*/
-const static_sir_channel_context_base_ptr : uint8_ptr_t;
-axiom static_sir_channel_context_base_ptr == 40960bv64;
+var recv_buf: mem_t; //from 413696bv64 to 417792bv64
+const recv_buf_size: uint64_t;        axiom recv_buf_size == 4096bv64;
+const recv_buf_ptr_low: uint8_ptr_t;  axiom recv_buf_ptr_low == 413696bv64;
+const recv_buf_ptr_high: uint64_t;    axiom recv_buf_ptr_high == 417792bv64;
+function {:inline} AddrInRecvBuf(ptr: bv64): bool { GE_64(ptr, recv_buf_ptr_low) && LT_64(ptr, recv_buf_ptr_high) }
 
-const stack_ptr_low: uint8_ptr_t;
-axiom stack_ptr_low == 8192bv64;
+/*************** SIR ****************/
+const SIR_ptr_high : uint8_ptr_t;     axiom SIR_ptr_high == 409600bv64;
 
-const stack_ptr_high: uint8_ptr_t;
-axiom stack_ptr_high == 12288bv64;
+var U: mem_t; //from 368640bv64 to 409600bv64
+const U_ptr_low : uint8_ptr_t;        axiom U_ptr_low == 368640bv64;
+const U_ptr_high : uint8_ptr_t;       axiom U_ptr_high == 409600bv64;
+function {:inline} AddrInU(ptr: bv64): bool { GE_64(ptr, U_ptr_low) && LT_64(ptr, U_ptr_high) }
 
-function {:inline} AddrInStack(rsp: bv64): bool
-{
-  GE_64(rsp, stack_ptr_low) && LT_64(rsp, stack_ptr_high)
-}
+/*************** lot of empty space ****************/
 
-const stack_guard_ptr_low: uint8_ptr_t;
-axiom stack_guard_ptr_low == 4096bv64;
+var symmetric_key: mem_t; //from 45056bv64 to 45088bv64
+const symmetric_key_ptr_low: uint8_ptr_t;                axiom symmetric_key_ptr_low == 45056bv64;
+const symmetric_key_ptr_high: uint8_ptr_t;               axiom symmetric_key_ptr_high == 45088bv64;
 
-const stack_guard_ptr_high: uint8_ptr_t;
-axiom stack_guard_ptr_high == 8192bv64;
+var sir_channel_context: mem_t; //40960bv64 to 41016bv64
+const sir_channel_context_ptr_low : uint8_ptr_t;  axiom sir_channel_context_ptr_low == 40960bv64;
+const sir_channel_context_ptr_high : uint8_ptr_t; axiom sir_channel_context_ptr_high == 41016bv64;
 
-const send_buf_ptr_low: uint8_ptr_t;
-axiom send_buf_ptr_low == 417792bv64;
-const send_buf_size: uint64_t;
-axiom send_buf_size == 4096bv64;
+/*************** lot of empty space ****************/
 
-const recv_buf_ptr_low: uint8_ptr_t;
-axiom recv_buf_ptr_low == 413696bv64;
-const recv_buf_size: uint64_t;
-axiom recv_buf_size == 4096bv64;
+var stack: mem_t; //from 8192bv64 to 12288bv64
+const stack_ptr_low: uint8_ptr_t;        axiom stack_ptr_low == 8192bv64;
+const stack_ptr_high: uint8_ptr_t;       axiom stack_ptr_high == 12288bv64;
+function {:inline} AddrInStack(rsp: bv64): bool { GE_64(rsp, stack_ptr_low) && LT_64(rsp, stack_ptr_high) }
 
-const symmetric_key_ptr_low: uint8_ptr_t;
-axiom symmetric_key_ptr_low == 45056bv64;
+var stack_guard: mem_t; //from 4096bv64 to 8192bv64
+const stack_guard_ptr_low: uint8_ptr_t;  axiom stack_guard_ptr_low == 4096bv64;
+const stack_guard_ptr_high: uint8_ptr_t; axiom stack_guard_ptr_high == 8192bv64;
+function {:inline} AddrInStackGuard(rsp: bv64): bool { GE_64(rsp, stack_guard_ptr_low) && LT_64(rsp, stack_guard_ptr_high) }
 
-const U_ptr_low: uint8_ptr_t;
-axiom U_ptr_low == 368640bv64;
-const U_ptr_high : uint8_ptr_t;
-axiom U_ptr_high == 409600bv64;
 
-const SIR_ptr_low: uint8_ptr_t;
-axiom SIR_ptr_low == 0bv64;
-const SIR_ptr_high : uint8_ptr_t;
-axiom SIR_ptr_high == 409600bv64;
+const SIR_ptr_low: uint8_ptr_t;          axiom SIR_ptr_low == 4096bv64;
+function {:inline} AddrInSIR(ptr: bv64): bool { GE_64(ptr, SIR_ptr_low) && LT_64(ptr, SIR_ptr_high) }
 
-function {:inline} AddrInU(ptr: bv64): bool
-{
-  GE_64(ptr, U_ptr_low) && LT_64(ptr, U_ptr_high)
-}
-
-function {:inline} AddrInSIR(ptr: bv64): bool
-{
-  GE_64(ptr, SIR_ptr_low) && LT_64(ptr, SIR_ptr_high)
-}
-
-function {:inline} get_send_buf_current(mem: mem_t): uint8_ptr_t
-{
-  LOAD_LE_64(mem, PLUS_64(static_sir_channel_context_base_ptr, 16bv64))
-}
-
-function {:inline} AddrInSendBuf(ptr: bv64): bool
-{
-  GE_64(ptr, send_buf_ptr_low) && LT_64(ptr, PLUS_64(send_buf_ptr_low, send_buf_size))
-}
+/*************** SIR ****************/
