proof/channel.bpl
@@ -30,22 +30,29 @@ function{:constructor} sir_channel_context_t( send_buf_start: uint8_ptr_t,
                        sir_channel_context_t;
 
 procedure {:inline 1} write_channel_context(ctx: sir_channel_context_t)
-modifies mem;
+modifies sir_channel_context;
 {
-  mem := STORE_LE_64(mem, PLUS_64(static_sir_channel_context_base_ptr, 0bv64),
-                          send_buf_start#sir_channel_context_t(ctx));
-  mem := STORE_LE_64(mem, PLUS_64(static_sir_channel_context_base_ptr, 8bv64),
-                          send_buf_size#sir_channel_context_t(ctx));
-  mem := STORE_LE_64(mem, PLUS_64(static_sir_channel_context_base_ptr, 16bv64),
-                          send_buf_current#sir_channel_context_t(ctx));
-  mem := STORE_LE_64(mem, PLUS_64(static_sir_channel_context_base_ptr, 24bv64),
-                          recv_buf_start#sir_channel_context_t(ctx));
-  mem := STORE_LE_64(mem, PLUS_64(static_sir_channel_context_base_ptr, 32bv64),
-                          recv_buf_size#sir_channel_context_t(ctx));
-  mem := STORE_LE_64(mem, PLUS_64(static_sir_channel_context_base_ptr, 40bv64),
-                          recv_buf_current#sir_channel_context_t(ctx));
-  mem := STORE_LE_64(mem, PLUS_64(static_sir_channel_context_base_ptr, 48bv64),
-                          symmetric_key#sir_channel_context_t(ctx));
+  sir_channel_context := STORE_LE_64(sir_channel_context,
+                                     PLUS_64(sir_channel_context_ptr_low, 0bv64),
+                                     send_buf_start#sir_channel_context_t(ctx));
+  sir_channel_context := STORE_LE_64(sir_channel_context,
+                                     PLUS_64(sir_channel_context_ptr_low, 8bv64),
+                                     send_buf_size#sir_channel_context_t(ctx));
+  sir_channel_context := STORE_LE_64(sir_channel_context,
+                                     PLUS_64(sir_channel_context_ptr_low, 16bv64),
+                                     send_buf_current#sir_channel_context_t(ctx));
+  sir_channel_context := STORE_LE_64(sir_channel_context,
+                                     PLUS_64(sir_channel_context_ptr_low, 24bv64),
+                                     recv_buf_start#sir_channel_context_t(ctx));
+  sir_channel_context := STORE_LE_64(sir_channel_context,
+                                     PLUS_64(sir_channel_context_ptr_low, 32bv64),
+                                     recv_buf_size#sir_channel_context_t(ctx));
+  sir_channel_context := STORE_LE_64(sir_channel_context,
+                                     PLUS_64(sir_channel_context_ptr_low, 40bv64),
+                                     recv_buf_current#sir_channel_context_t(ctx));
+  sir_channel_context := STORE_LE_64(sir_channel_context,
+                                     PLUS_64(sir_channel_context_ptr_low, 48bv64),
+                                     symmetric_key#sir_channel_context_t(ctx));
 }
 
 /*
@@ -58,14 +65,19 @@ type{:datatype} sir_message_header_t;
 function{:constructor} sir_message_header_t (message_type: uint64_t,
                                              message_size: uint64_t) :
                        sir_message_header_t;
+
 procedure {:inline 1} write_message_header(ptr: uint8_ptr_t,
                                            hdr: sir_message_header_t)
-modifies mem;
+modifies send_buf;
 {
-  mem := STORE_LE_64(mem, PLUS_64(ptr, 0bv64),
-                         message_type#sir_message_header_t(hdr));
-  mem := STORE_LE_64(mem, PLUS_64(ptr, 8bv64),
-                         message_size#sir_message_header_t(hdr));
+  assert AddrInSendBuf(ptr) && AddrInSendBuf(PLUS_64(ptr, 15bv64));
+
+  send_buf := STORE_LE_64(send_buf,
+                          PLUS_64(ptr, 0bv64),
+                          message_type#sir_message_header_t(hdr));
+  send_buf := STORE_LE_64(send_buf,
+                          PLUS_64(ptr, 8bv64),
+                          message_size#sir_message_header_t(hdr));
 }
 
 procedure {:inline 1} init_channel( send_buf_start: uint8_ptr_t,
@@ -73,16 +85,16 @@ procedure {:inline 1} init_channel( send_buf_start: uint8_ptr_t,
                                     recv_buf_start: uint8_ptr_t,
                                     recv_buf_size: uint64_t,
                                     symmetric_key: uint64_t )
-modifies mem;
+modifies sir_channel_context;
 {
   var tmp: sir_channel_context_t;
   tmp  :=  sir_channel_context_t(send_buf_start,
-                               send_buf_size,
-                               send_buf_start,
-                               recv_buf_start,
-                               recv_buf_size,
-                               recv_buf_start,
-                               symmetric_key);
+                                 send_buf_size,
+                                 send_buf_start,
+                                 recv_buf_start,
+                                 recv_buf_size,
+                                 recv_buf_start,
+                                 symmetric_key);
   call write_channel_context(tmp);
 }
 
@@ -93,22 +105,32 @@ returns (result: bool)
   var send_buf_size: uint8_ptr_t;
   var send_buf_start: uint8_ptr_t;
 
-  send_buf_start   := LOAD_LE_64(mem, PLUS_64(static_sir_channel_context_base_ptr, 0bv64));
-  send_buf_size    := LOAD_LE_64(mem, PLUS_64(static_sir_channel_context_base_ptr, 8bv64));
-  send_buf_current := LOAD_LE_64(mem, PLUS_64(static_sir_channel_context_base_ptr, 16bv64));
+  send_buf_start   := LOAD_LE_64(sir_channel_context,
+                                 PLUS_64(sir_channel_context_ptr_low, 0bv64));
+  send_buf_size    := LOAD_LE_64(sir_channel_context,
+                                 PLUS_64(sir_channel_context_ptr_low, 8bv64));
+  send_buf_current := LOAD_LE_64(sir_channel_context,
+                                 PLUS_64(sir_channel_context_ptr_low, 16bv64));
 
-  result := LT_64(PLUS_64(send_buf_current, size), PLUS_64(send_buf_start, send_buf_size)) &&
+  result := LE_64(PLUS_64(send_buf_current, size), PLUS_64(send_buf_start, send_buf_size)) &&
             GE_64(PLUS_64(send_buf_current, size), send_buf_current);
 }
 
-procedure {:inline 1} channel_send( msg_typ: uint64_t,
-                        msg_buf: uint8_ptr_t,
-                        msg_size: uint64_t )
+procedure {:inline 1} channel_send( msg_typ : uint64_t,
+                                    msg_buf : uint8_ptr_t,
+                                    msg_size: uint64_t )
 returns (result: channel_api_result_t)
-modifies mem;
+requires AddrInSendBuf(LOAD_LE_64(sir_channel_context,
+                                  PLUS_64(sir_channel_context_ptr_low, 16bv64)));
+ensures AddrInSendBuf(LOAD_LE_64(sir_channel_context,
+                                  PLUS_64(sir_channel_context_ptr_low, 16bv64)));
+
+modifies send_buf, stack, sir_channel_context;
 {
   var msg_header: sir_message_header_t; //ghost_var
   var send_buf_current: uint8_ptr_t;    //ghost_var
+  var send_buf_size: uint8_ptr_t;    //ghost_var
+  var send_buf_start: uint8_ptr_t;    //ghost_var
   var space_available : bool; //ghost var
 
   var msg_header_base_ptr: uint8_ptr_t;
@@ -117,35 +139,60 @@ modifies mem;
   //rsp is arbitrary at the time of call.
   havoc rsp; assume AddrInStack(rsp);
   //sir_message_header_t msg_header; resides on the stack
+  rsp := MINUS_64(rsp, 16bv64);
   msg_header_base_ptr := rsp;
   //msg_header.message_type = type; msg_header.message_size = size;
-  call havoc_region(msg_header_base_ptr, 16bv64);
+  stack := STORE_LE_64(stack, PLUS_64(msg_header_base_ptr, 0bv64), msg_typ);
+  stack := STORE_LE_64(stack, PLUS_64(msg_header_base_ptr, 8bv64), msg_size);
+
+  //compute ghost vars
+  send_buf_current := LOAD_LE_64(sir_channel_context,
+                                 PLUS_64(sir_channel_context_ptr_low, 16bv64));
 
   //  if (!bytes_available_in_send_buf(size + sizeof(sir_message_header_t))) {
   //    return CHANNEL_FAILURE;
   //  }
   call space_available := bytes_available_in_send_buf(PLUS_64(msg_size, 16bv64));
   if (!space_available) {
+    assume false;
+    assume AddrInSendBuf(send_buf_current);
     result := channel_failure; return;
   }
 
-  //compute ghost vars
-  send_buf_current := LOAD_LE_64(mem, PLUS_64(static_sir_channel_context_base_ptr, 16bv64));
+
   msg_header := sir_message_header_t(msg_typ, msg_size);
+
+  assume LE_64(msg_size, 128bv64);
+  assume AddrInSendBuf(send_buf_current) &&
+         AddrInSendBuf(PLUS_64(send_buf_current, 15bv64)) &&
+         LE_64(send_buf_current, PLUS_64(send_buf_current, 15bv64));
+  assume AddrInSendBuf(send_buf_current) &&
+         AddrInSendBuf(PLUS_64(send_buf_current, PLUS_64(msg_size,15bv64))) &&
+         LE_64(send_buf_current, PLUS_64(send_buf_current, PLUS_64(msg_size,15bv64)));
+  //assert AddrInSendBuf(PLUS_64(PLUS_64(send_buf_current, 15bv64), msg_size));
 
   //memcpy(sir_channel_context.send_buf_current, &msg_header, sizeof(msg_header));
   call write_message_header(send_buf_current, msg_header);
   //sir_channel_context.send_buf_current += sizeof(msg_header);
   send_buf_current := PLUS_64(send_buf_current, 16bv64); //sizeof(msg_header_t) = 16
-  mem := STORE_LE_64(mem, PLUS_64(static_sir_channel_context_base_ptr, 16bv64),
-                          send_buf_current); //sizeof(msg_header_t) = 16
+  sir_channel_context := STORE_LE_64(sir_channel_context,
+                                     PLUS_64(sir_channel_context_ptr_low, 16bv64),
+                                     send_buf_current); //sizeof(msg_header_t) = 16
 
+  assume AddrInSendBuf(send_buf_current) &&
+         AddrInSendBuf(PLUS_64(send_buf_current, MINUS_64(msg_size,1bv64))) &&
+         LE_64(send_buf_current, PLUS_64(send_buf_current, MINUS_64(msg_size,1bv64)));
   //memcpy(sir_channel_context.send_buf_current, buf, size);
-  call memcpy(send_buf_current, msg_buf, msg_size);
+  call send_buf_memcpy(send_buf_current, msg_buf, msg_size);
   //sir_channel_context.send_buf_current += size;
   send_buf_current := PLUS_64(send_buf_current, msg_size);
-  mem := STORE_LE_64(mem, PLUS_64(static_sir_channel_context_base_ptr, 16bv64),
-                          send_buf_current); //sizeof(msg_header_t)
+  if (send_buf_ptr_high == send_buf_current)
+  {
+    send_buf_current := send_buf_ptr_low;
+  }
+  sir_channel_context := STORE_LE_64(sir_channel_context,
+                                     PLUS_64(sir_channel_context_ptr_low, 16bv64),
+                                     send_buf_current); //sizeof(msg_header_t)
 
   //yield: adversary havocs non-SIR memory
   //call havoc_non_sir_region(); //registers are preserved
@@ -156,9 +203,9 @@ modifies mem;
 
 procedure L_send( msg_buf: uint8_ptr_t, msg_size: uint64_t )
 returns (result: channel_api_result_t)
-requires AddrInSendBuf(get_send_buf_current(mem));
-ensures  AddrInSendBuf(get_send_buf_current(mem));
-modifies mem;
+requires AddrInSendBuf(LOAD_LE_64(sir_channel_context, PLUS_64(sir_channel_context_ptr_low, 16bv64)));
+ensures  AddrInSendBuf(LOAD_LE_64(sir_channel_context, PLUS_64(sir_channel_context_ptr_low, 16bv64)));
+modifies send_buf, stack, sir_channel_context;
 {
   var symmetric_key_ptr:  uint8_ptr_t; //ghost var
 
@@ -168,14 +215,15 @@ modifies mem;
 
   //rsp is arbitrary at the time of call.
   havoc rsp; assume AddrInStack(rsp);
+  rsp := MINUS_64(rsp, 288bv64);
   //uint8_t buf_128_bytes[128]; resides on the stack
-  buf_128_bytes_ptr := rsp;
+  buf_128_bytes_ptr := PLUS_64(rsp,160bv64);
   //uint8_t ciphertext[160]; resides on the stack
-  ciphertext_ptr := MINUS_64(rsp, 128bv64);
+  ciphertext_ptr := rsp;
 
   //TODO: fix this in the code
   if (! (AddrInU(msg_buf) &&
-         AddrInU(PLUS_64(msg_buf,msg_size)) &&
+         AddrInU(PLUS_64(msg_buf,MINUS_64(msg_size,1bv64))) &&
          LE_64(msg_buf, PLUS_64(msg_buf,msg_size))) )
   {
     result := channel_failure;
@@ -191,23 +239,24 @@ modifies mem;
   // if (sir_channel_context.symmetric_key == NULL) {
   //   return channel_send(SEND_MESSAGE, buf, size);
   // }
-  symmetric_key_ptr := LOAD_LE_64(mem, PLUS_64(static_sir_channel_context_base_ptr, 64bv64));
+  symmetric_key_ptr := LOAD_LE_64(sir_channel_context,
+                                  PLUS_64(sir_channel_context_ptr_low, 64bv64));
   if (symmetric_key_ptr == NULL) {
     call result := channel_send(0bv64, msg_buf, msg_size);
     return;
   }
 
   // memset(buf_128_bytes, 0x00, sizeof(buf_128_bytes));
-  call memset(buf_128_bytes_ptr, 0bv8, 128bv64);
+  call stack_memset(buf_128_bytes_ptr, 0bv8, 128bv64);
   // memcpy(buf_128_bytes, buf, size);
-  call memcpy(buf_128_bytes_ptr, msg_buf, msg_size);
+  call stack_memcpy(buf_128_bytes_ptr, msg_buf, msg_size);
 
   //rng_result = rdrand_get_bytes(16, ciphertext + 128);
   //if (rng_result != DRNG_SUCCESS) { exit(1); }
-  call havoc_region(PLUS_64(ciphertext_ptr, 128bv64), 16bv64);
+  call havoc_stack_region(PLUS_64(ciphertext_ptr, 128bv64), 16bv64);
 
   //aes_result = aes_gcm_encrypt_and_tag(..)
-  call havoc_region(ciphertext_ptr, 160bv64);
+  call havoc_stack_region(ciphertext_ptr, 160bv64);
 
   //send_result = channel_send(SEND_ENCRYPTED_MESSAGE, ciphertext, 160);
   call result := channel_send(0bv64, ciphertext_ptr, 160bv64);
@@ -217,7 +266,6 @@ modifies mem;
 
 procedure L_recv( msg_buf: uint8_ptr_t, msg_size: uint64_t )
 returns (result: channel_api_result_t)
-modifies mem;
 {
   result := channel_failure;
 }
