proof/heap.bpl
@@ -1,12 +1,12 @@
 procedure L_malloc( size: uint64_t )
 //returns (result: uint8_ptr_t)
-modifies mem;
+//modifies mem;
 {
 
 }
 
 procedure L_free( buf: uint8_ptr_t )
-modifies mem;
+//modifies mem;
 {
 
 }
