proof/verified_L.bpl
@@ -1,5 +1,5 @@
 procedure main()
-modifies mem;
+modifies send_buf, recv_buf, stack, stack_guard, sir_channel_context, symmetric_key, U;
 {
   var buf: uint8_ptr_t;
   var size: uint64_t;
@@ -8,9 +8,9 @@ modifies mem;
   call init_channel(send_buf_ptr_low, send_buf_size,
                     recv_buf_ptr_low, recv_buf_size,
                     symmetric_key_ptr_low);
-                    
+
   while(*)
-  invariant AddrInSendBuf(get_send_buf_current(mem));
+  invariant AddrInSendBuf(LOAD_LE_64(sir_channel_context, PLUS_64(sir_channel_context_ptr_low, 16bv64)));
   {
     havoc buf;
     havoc size;
